wip

lawyer/nonblocking/tokens/wfree_adequacy_tokens.v
@@ -8,6 +8,7 @@ From lawyer Require Import program_logic sub_action_em action_model.
 From lawyer.examples Require Import orders_lib obls_tactics.
 From lawyer.nonblocking Require Import trace_context om_wfree_inst pr_wfree_lib (* pr_wfree *) wfree_traces wptp_gen pwp calls wfree_adequacy_lib.
 (* From lawyer.nonblocking.logrel Require Import fundamental.  *)
+From lawyer.nonblocking.logrel Require Import valid_client.
 From lawyer.nonblocking.tokens Require Import om_wfree_inst_tokens.
 From lawyer.obligations Require Import obligations_resources obligations_logic env_helpers obligations_adequacy obligations_model obligations_em obligations_am obls_termination.
 From heap_lang Require Import lang simulation_adequacy.
@@ -45,6 +46,204 @@ Section WFAdequacy.
 
   Let fic := fits_inf_call ic m ai.
 
+  Definition is_init_tpool (tp: list expr) :=
+    Forall (fun e => exists e0, e = subst "m" m e0 /\ valid_client e0) tp /\
+    (ii = 0 -> exists e, from_locale tp τi = Some e /\ under_ctx Ki e = Some (m ai)) /\
+    (forall e, from_locale tp τi = Some e -> to_val e = None).
+
+  Definition obls_om_traces_match_wfree: extrace heap_lang -> trace (mstate M) (mlabel M) -> Prop :=
+    obls_om_traces_match_gen (obls_st_rel_wfree ic). 
+
+  Theorem om_simulation_adequacy_model_trace_multiple_waitfree Σ
+        `{hPre: @heapGpreS Σ M EM} (s: stuckness)
+        (es: list expr) σ1 (s1: mstate M) p
+        (INIT: em_is_init_st (es, σ1) s1 (ExecutionModel := EM))
+        (extr : extrace heap_lang)
+        (Hvex : extrace_valid extr)
+        (Hexfirst : trfirst extr = (es, σ1))
+    :
+    PR_premise_multiple (obls_sim_rel_wfree ic s') (fits_inf_call ic m ai) Σ s es σ1 s1 (p: @em_init_param _ _ EM) ->
+    (∃ omtr, obls_om_traces_match_wfree extr omtr ∧ trfirst omtr = s1 /\
+              int_ref_inf (obls_sim_rel_wfree ic s') extr omtr
+    ) \/
+    (exists k, ¬ (fits_inf_call ic m ai) (trace_take_fwd k extr)).
+  Proof using. Admitted. 
+
+  Definition wfreeΣ: gFunctors := iemΣ HeapLangEM EM. 
+
+  Instance wfree_pre: @heapGpreS wfreeΣ M EM.
+  Proof. 
+    unshelve esplit. 
+  Qed. 
+
+  Lemma PR_premise_wfree `{hPre: @heapGpreS Σ M EM} c
+    (ETR0: is_init_tpool c.1)
+    (MOD_INIT: wfst_is_init_st _ SPEC c)
+    (M_FUN: is_fun m)
+    :
+  PR_premise_multiple (obls_sim_rel_wfree ic s') (fits_inf_call ic m ai)
+    Σ MaybeStuck c.1 c.2
+    (init_om_wfree_state F ic c) ((): @em_init_param _ _ EM).
+  Proof using. Admitted.
+
+  (* TODO: rename *)
+  Lemma simple_om_simulation_adequacy_terminate_multiple_waitfree_impl extr
+    (MOD_INIT : wfst_is_init_st _ SPEC (trfirst extr))
+    (VALID : extrace_valid extr)
+    (FAIR : fair_call extr tpc ii)
+    (INIT_TP : is_init_tpool (trfirst extr).1)
+    (CALL: from_option (fun c => call_at tpc c m ai (APP := App)) False (extr S!! ii))
+    (M_FUN: is_fun m):
+    terminating_trace extr /\ int_ref_inf_one (call_progresses ic s') extr ∨
+    (∃ k, ¬ fits_inf_call ic m ai (trace_take_fwd k extr)) \/
+    (s' = MaybeStuck /\ gets_stuck_ae extr ic). 
+  Proof using.
+    clear MSm.
+    opose proof (om_simulation_adequacy_model_trace_multiple_waitfree
+                wfreeΣ _ (trfirst extr).1 _ _ _ _ _ VALID _ _) as ADEQ.
+    { apply init_om_wfree_is_init. }
+    { apply surjective_pairing. }     
+    { rewrite -surjective_pairing. 
+      eapply PR_premise_wfree; eauto. }
+    
+    destruct ADEQ as [(mtr & MATCH & OM0 & IREF) | RET].
+    2: { right. left. done. } 
+
+    opose proof (obls_matching_traces_OM _ _ _ _ MATCH _) as (omtr & MATCH'' & SR & OM_WF & FIRST'').
+    { intros ?? X. apply X. }
+    { eapply obls_init_wf. rewrite OM0. apply init_om_wfree_is_init. }
+
+    destruct (Classical_Prop.classic (∃ j, has_return_at extr ic j)) as [[j RET]| NORET].
+    { red in RET. rewrite (ic_helper ic) in RET.
+      destruct RET as (r & cj & ? & JTH & RET).
+      right. left. exists j. intros [_ NVALS _]. 
+      specialize (NVALS _ H).
+
+      eapply trace_take_fwd_lookup_Some' in JTH.
+      2: reflexivity.
+      rewrite JTH /= in NVALS.
+      edestruct not_return_nval; eauto. }
+
+    assert (int_ref_inf_one (call_progresses ic s') extr) as IREF1.
+    { eapply int_ref_inf_proj_one. eapply int_ref_inf_impl; eauto.
+      by intros ?? (?&?&?). }
+
+    destruct (extr S!! ii) as [ci | ] eqn:IITH.
+    2: { left.
+         pose proof (trace_has_len extr) as [??]. 
+         eapply state_lookup_dom_neg in IITH; eauto.
+         split; [| done].
+         eapply terminating_trace_equiv; eauto.
+         destruct x; try done. }
+
+    add_case (exists N, ii <= N /\ is_Some (extr S!! N) /\ ∀ j, N ≤ j → from_option (not_stuck_tid τi) True (extr S!! j)) IF_NS. 
+    { intros NS. 
+    
+      assert (forall τ, obls_trace_fair τ omtr) as OM_FAIR.
+      { eapply om_trace_fair; eauto. }
+
+      left. split; [| done]. 
+      pose proof (traces_match_valid2 _ _ _ _ _ _ MATCH'') as OM_VALID.
+      pose proof (obls_fair_trace_terminate _ OM_VALID OM_FAIR) as OM_TERM.
+      
+      eapply (traces_match_preserves_termination _ _ _ _ _ _ MATCH'').
+      apply OM_TERM; eauto.
+      + apply unit_WF.
+      + apply fin_wf. }
+
+    destruct (decide (s' = MaybeStuck)) as [S'|S']. 
+    2: { apply IF_NS. 
+         exists ii. split; [lia| ]. split; [done| ].
+         intros.
+         destruct (extr S!! j) eqn:ITH; [| done]. simpl.
+         eapply ref_call_progress_last; eauto. by destruct s'. }
+    
+    destruct (Classical_Prop.classic (gets_stuck_ae extr ic)) as [| NS]. 
+    { do 2 right. tauto. }
+    apply IF_NS.
+
+    rewrite /gets_stuck_ae in NS.
+    rewrite not_all_ex_not_iff in NS. destruct NS as (N & NS).
+    apply not_impl_and_not_iff in NS as ([? NTH] & NS).
+    exists (max ii N). split; [lia| ].
+    split.
+    { pose proof (Nat.max_spec_le ii N) as [[? MAX] | [? MAX]]; rewrite MAX; eauto. }
+    intros. destruct (extr S!! j) eqn:JTH; [| done]. simpl.
+    
+    rewrite not_ex_all_not_iff in NS.
+    specialize (NS j). rewrite /ge in NS. rewrite !not_and_l in NS.
+    destruct NS as [? | [? | NS]].
+    { lia. }
+    { set_solver. }
+    rewrite /gets_stuck_at /= in NS.
+    rewrite (ic_helper ic) /tpc (tc_helper ic) in NS.
+    rewrite JTH in NS.
+    destruct (decide (not_stuck_tid τi c)); [done| ]. destruct NS.
+    eexists. repeat split.
+    { lia. }
+    apply stuck_tid_neg. split; eauto.
+    opose proof * from_locale_trace.
+    { done. }
+    { apply IITH. }
+    { simpl in CALL.
+      move CALL at bottom. do 2 red in CALL.
+      rewrite /tpc tc_helper /= in CALL.
+      apply mk_is_Some in CALL. apply CALL. }
+    { etrans; [| apply H]. lia. }
+    by rewrite JTH in H0.
+  Qed.
+
+  Theorem simple_om_simulation_adequacy_terminate_multiple_waitfree extr
+        (ETR0: valid_init_tpool_restr (trfirst extr).1 ms)
+        (MOD_INIT: wfst_is_init_st _ SPEC (trfirst extr))
+        (CALL: from_option (fun c => call_at tpc c m ai (APP := App)) False (extr S!! ii))
+    :
+    extrace_valid extr -> 
+    fair_call extr tpc ii ->
+    (exists f x b, m = RecV f x b) ->
+    terminating_trace extr /\ int_ref_inf_one (call_progresses ic s') extr \/ 
+    (exists k, ¬ fits_inf_call ic m ai (trace_take_fwd k extr)) \/
+    (s' = MaybeStuck /\ gets_stuck_ae extr ic). 
+  Proof.
+    intros VALID FAIR M_FUN. 
+
+    destruct (decide (ii = 0 → ∃ e,
+                    from_locale (trfirst extr).1 τi = Some e ∧ under_ctx Ki e = Some (m ai))) as [II0| ].
+    2: { pose proof tc_helper. 
+         clear -n H.
+         right. left. 
+         apply Classical_Prop.imply_to_and in n as (II & NO0).
+         exists 0. intros FITS. apply NO0.
+         destruct FITS.
+         fold ii in fic_call.
+         rewrite trace_take_fwd_0_first in fic_call.
+         rewrite II /= in fic_call.
+         red in fic_call. simpl in fic_call. eauto.
+         red in fic_call. rewrite H in fic_call.
+         eexists. split; eauto. by rewrite under_ctx_fill. }
+
+    destruct (@decide (∀ e, from_locale (trfirst extr).1 τi = Some e → to_val e = None)) as [E0| ].
+    { destruct (from_locale (trfirst extr).1 τi) eqn:E.
+      2: { left. set_solver. }
+      destruct (to_val e) eqn:V.
+      { right. set_solver. }
+      left. set_solver. }
+    2: { apply not_forall_exists_not in n as [e VAL].
+         apply Classical_Prop.imply_to_and in VAL as [E VAL].
+         right. left. exists 0. intros FITS. apply VAL.
+         destruct FITS. 
+         specialize (fic_never_val 0). rewrite trace_take_fwd_0_first /= in fic_never_val.
+         rewrite E in fic_never_val. done. }
+
+    assert (is_init_tpool (trfirst extr).1) as INIT_TP.
+    { repeat split; eauto.
+      red in ETR0.
+      (* should follow from ETR0 *)
+      admit. }
+
+    by apply simple_om_simulation_adequacy_terminate_multiple_waitfree_impl.
+  Admitted.
+
   (* TODO: rename *)
   Lemma obls_terminates_impl_multiple_waitfree
     (extr : extrace heap_lang)
@@ -59,7 +258,15 @@ Section WFAdequacy.
     terminating_trace extr /\ int_ref_inf_one (call_progresses ic s') extr
     \/ has_return extr ic \/
     (s' = MaybeStuck /\ gets_stuck_ae extr ic). 
-  Proof. Admitted. 
+  Proof.
+    opose proof * (simple_om_simulation_adequacy_terminate_multiple_waitfree) as ADEQ; eauto.
+
+    destruct ADEQ as [| [[n NFIT] | STUCK]]; [tauto| | tauto]. 
+    right. left. red. simpl in *.
+    
+    destruct (extr S!! ii) as [ci | ] eqn:ITH; rewrite ITH /= in CALL; [| done].
+    by eapply not_fic_has_return.
+  Qed.
     
 End WFAdequacy.
 
