lawyer/nonblocking/wfree_adequacy_lib.v
@@ -773,3 +773,4 @@ Proof using.
   eapply mk_is_Some, state_lookup_dom in NEXT; eauto.
   simpl in *. lia.
 Qed.  
+
